Moved the code to automatically generate "boolify" functions for datatypes from src/datatype/Datatype.sml to src/Boolify/src/Boolify.sml.
It uses the register_update_function hook to add the boolification
info (more on that later).

Also added a test suite for boolification.

src/Boolify/src/Boolify.sig
@@ -1,0 +1,7 @@
+(* ========================================================================= *)
+(* AUTOMATICALLY WRITING BOOLIFICATION FUNCTIONS FOR DATATYPES.              *)
+(* Created by Joe Hurd, July 2002                                            *)
+(* Basically the same as Konrad Slind's code to generate size functions      *)
+(* ========================================================================= *)
+
+signature Boolify = sig end
