src/Boolify/src/Boolify.sml
@@ -1,0 +1,281 @@
+(* ========================================================================= *)
+(* AUTOMATICALLY WRITING BOOLIFICATION FUNCTIONS FOR DATATYPES.              *)
+(* Created by Joe Hurd, July 2002                                            *)
+(* Basically the same as Konrad Slind's code to generate size functions      *)
+(* ========================================================================= *)
+
+(*
+val () = loadPath := ["../../list/src"] @ !loadPath;
+*)
+
+(*
+*)
+structure Boolify :> Boolify =
+struct
+
+open HolKernel boolLib Parse pairSyntax numSyntax listSyntax
+  combinSyntax arithmeticTheory mesonLib simpLib boolSimps numLib
+  optionTheory listSyntax BoolifyTheory PreListBoolify;
+  
+infix 0 THEN |->;
+infixr 1 --> by;
+
+(* ------------------------------------------------------------------------- *)
+(* Helper functions.                                                         *)
+(* ------------------------------------------------------------------------- *)
+
+val ERR = mk_HOL_ERR "Boolify";
+
+val head = Lib.repeat rator;
+
+val bool_list = mk_list_type bool;
+
+val bool_nil = mk_thy_const {Thy = "list", Name = "NIL", Ty = bool_list};
+  
+val bool_cons =
+  mk_thy_const
+  {Thy = "list", Name = "CONS", Ty = bool --> bool_list --> bool_list};
+fun mk_bool_cons (x, y) = list_mk_comb (bool_cons, [x, y]);
+  
+val bool_append =
+  mk_thy_const
+  {Thy = "list", Name = "APPEND",
+   Ty = bool_list --> bool_list --> bool_list};
+fun mk_bool_append (x, y) = list_mk_comb (bool_append, [x, y]);
+
+(*---------------------------------------------------------------------------
+   A tyspec is a type specification.  The first component is a type
+   variable whose name (less the leading quote) is the name of the new
+   type.  Each such is accompanied by a list of constructor specifications.
+   Such a spec. is a string (the constructor name) and a list of types that
+   are the arguments of that constructor.  Recursive occurrences of the
+   types are marked by occurrences of the corresponding type variables.
+ ---------------------------------------------------------------------------*)
+
+local open Portable
+      fun num_variant vlist v =
+        let val counter = ref 0
+            val names = map (fst o dest_var) vlist
+            val (Name,Ty) = dest_var v
+            fun pass str =
+               if mem str names
+               then (inc counter; pass (Name^Lib.int_to_string(!counter)))
+               else str
+        in mk_var(pass Name,  Ty)
+        end
+in
+fun mk_tyvar_boolify vty (V,away) =
+  let val fty = vty --> mk_type ("list", [bool])
+      val v = num_variant away (mk_var("f", fty))
+  in (v::V, v::away)
+  end
+end;
+
+fun tyboolify_env db = 
+     Option.map fst o 
+     Option.composePartial (TypeBasePure.boolify_of, TypeBasePure.get db)
+
+(*---------------------------------------------------------------------------*
+  Term boolification, another type-based translation.
+ *---------------------------------------------------------------------------*)
+
+fun bool_lists n =
+  let
+    val ConsT = curry mk_bool_cons T
+    val ConsF = curry mk_bool_cons F
+    fun booll 0 = [bool_nil]
+      | booll n = let val l = booll (n div 2) in map ConsT l @ map ConsF l end
+  in
+    List.take (booll (n - 1), n)
+  end;
+
+local fun drop [] ty = fst(dom_rng ty)
+        | drop (_::t) ty = drop t (snd(dom_rng ty));
+      fun Kzero ty = mk_abs (mk_var ("v", ty), bool_nil)
+      fun OK f ty M =
+         let val (Rator,Rand) = dest_comb M
+         in (Rator=f) andalso is_var Rand andalso (type_of Rand = ty)
+         end
+in
+fun tyboolify (theta,omega,gamma) clause ty =
+ case theta ty
+  of SOME fvar => fvar
+   | NONE =>
+      case omega ty
+       of SOME (_,[]) => raise ERR "tyboolify" "bug: no assoc for nested"
+        | SOME (_,[(f,szfn)]) => szfn
+        | SOME (_,alist) => snd
+             (first (fn (f,sz) => Lib.can (find_term(OK f ty)) (rhs clause))
+                  alist)
+        | NONE =>
+           let val (Tyop,Args) = dest_type ty
+           in case gamma Tyop
+               of SOME f =>
+                   let val vty = drop Args (type_of f)
+                       val sigma = Type.match_type vty ty
+                    in list_mk_comb(inst sigma f,
+                                map (tyboolify (theta,omega,gamma) clause) Args)
+                    end
+                | NONE => Kzero ty
+             end
+
+fun type_boolify db ty =
+  let fun theta ty = if is_vartype ty then SOME (Kzero ty) else NONE
+      fun omega ty = NONE
+  in
+    tyboolify (theta,omega,tyboolify_env db) ty
+  end
+end;
+
+fun dupls [] (C,D) = (rev C, rev D)
+  | dupls (h::t) (C,D) = dupls t (if mem h t then (C,h::D) else (h::C,D));
+
+fun crunch [] = []
+  | crunch ((x,y)::t) =
+    let val key = #1(dom_rng(type_of x))
+        val (yes,no) = partition (fn(x,_) => (#1(dom_rng(type_of x))=key)) t
+    in (key, (x,y)::yes)::crunch no
+    end;
+
+fun unflatten f =
+  let
+    fun h (x, s) =
+      let
+        val k = f x
+      in
+        case List.partition (equal k o fst) s of ([(_, l)], r)
+          => (k, x :: l) :: r
+        | _ => (k, [x]) :: s
+      end
+  in
+    rev o map (rev o snd) o foldl h []
+  end;
+
+fun define_boolify ax db =
+ let val dtys = Prim_rec.doms_of_tyaxiom ax  (* primary types in axiom *)
+     val tyvars = Lib.U (map (snd o dest_type) dtys)
+     val (_, abody) = strip_forall(concl ax)
+     val (exvs, ebody) = strip_exists abody
+     (* list of all constructors with arguments *)
+     val conjl = strip_conj ebody
+     val bare_conjl = map (snd o strip_forall) conjl
+     val capplist = map (rand o lhs) bare_conjl
+     val def_name = fst(dest_type(type_of(hd capplist)))
+     (* 'a -> bool list variables : boolify functions for type variables *)
+     val fparams = rev(fst(rev_itlist mk_tyvar_boolify tyvars
+                             ([],free_varsl capplist)))
+     val fparams_tyl = map type_of fparams
+     fun proto_const n ty =
+         mk_var(n, itlist (curry op-->) fparams_tyl (ty --> bool_list))
+     fun tyop_binding ty =
+       let val root_tyop = fst(dest_type ty)
+       in (root_tyop, (ty, proto_const(root_tyop^"_to_bool") ty))
+       end
+     val tyvar_map = zip tyvars fparams
+     val tyop_map = map tyop_binding dtys
+     fun theta tyv =
+          case assoc1 tyv tyvar_map
+           of SOME(_,f) => SOME f
+            | NONE => NONE
+     val type_boolify_env = tyboolify_env db
+     fun gamma str =
+          case assoc1 str tyop_map
+           of NONE  => type_boolify_env str
+            | SOME(_,(_, v)) => SOME v
+     (* now the ugly nested map *)
+     val head_of_clause = head o lhs o snd o strip_forall
+     fun is_dty M = mem(#1(dom_rng(type_of(head_of_clause M)))) dtys
+     val (dty_clauses,non_dty_clauses) = partition is_dty bare_conjl
+     val dty_fns = fst(dupls (map head_of_clause dty_clauses) ([],[]))
+     fun dty_boolify ty =
+        let val (d,r) = dom_rng ty
+        in list_mk_comb(proto_const(fst(dest_type d)^"_to_bool") d,fparams)
+        end
+     val dty_map = zip dty_fns (map (dty_boolify o type_of) dty_fns)
+     val non_dty_fns = fst(dupls (map head_of_clause non_dty_clauses) ([],[]))
+     fun nested_binding (n,f) =
+        let val name = String.concat[def_name,Lib.int_to_string n,"_to_bool"]
+            val (d,r) = dom_rng (type_of f)
+            val proto_const = proto_const name d
+        in (f, list_mk_comb (proto_const,fparams))
+       end
+     val nested_map0 = map nested_binding (enumerate 1 non_dty_fns)
+     val nested_map1 = crunch nested_map0
+     fun omega ty = assoc1 ty nested_map1
+     val boolifyr = tyboolify(theta,omega,gamma)
+     fun mk_app cl v = mk_comb(boolifyr cl (type_of v), v)
+     val fn_i_map = dty_map @ nested_map0
+     fun clause (bl, cl) =
+         let val (fn_i, capp) = dest_comb (lhs cl)
+         in
+         mk_eq(mk_comb(assoc fn_i fn_i_map, capp),
+               end_itlist (curry mk_bool_append)
+               (bl :: map (mk_app cl) (snd(strip_comb capp))))
+(*
+               case snd(strip_comb capp)
+                of [] => bool_nil ()
+                 | L  => end_itlist (curry mk_bool_append)
+                         (mk_bool_cons (T, bool_nil ())::map (mk_app cl) L))
+*)
+         end
+     val bare_conjls = unflatten (rator o lhs) bare_conjl
+     val annot_conjs =
+       flatten (map (fn l => zip (bool_lists (length l)) l) bare_conjls)
+     val pre_defn0 = list_mk_conj (map clause annot_conjs)
+     val nil_rws =
+       [CONJUNCT1 (DB.fetch "list" "APPEND"), DB.fetch "list" "APPEND_NIL"]
+     val pre_defn1 = rhs(concl   (* remove zero additions *)
+                      ((DEPTH_CONV BETA_CONV THENC
+                        Rewrite.PURE_REWRITE_CONV nil_rws) pre_defn0))
+     val defn = new_recursive_definition
+                 {name=def_name^"_to_bool_def",
+                  rec_axiom=ax, def=pre_defn1}
+     val cty = (I##(type_of o last)) o strip_comb o lhs o snd o strip_forall
+     val ctyl = Lib.mk_set (map cty (strip_conj (concl defn)))
+     val const_tyl = gather (fn (c,ty) => mem ty dtys) ctyl
+     val const_tyopl = map (fn (c,ty) => (c,fst(dest_type ty))) const_tyl
+ in
+    SOME {def=defn,const_tyopl=const_tyopl}
+ end
+ handle HOL_ERR _ => NONE;
+
+(*---------------------------------------------------------------------------
+      Writing all the boolification information to the typebase.
+ ---------------------------------------------------------------------------*)
+
+fun insert_boolify {def, const_tyopl} tyinfol =
+  (case tyinfol of [] => raise ERR "build_tyinfos" "empty tyinfo list"
+   | tyinfo::rst =>
+     let
+       val first_tyname = TypeBasePure.ty_name_of tyinfo
+       fun ins_boolify info boolify_eqs =
+         let
+           val tyname = TypeBasePure.ty_name_of info
+         in
+           case assoc2 tyname const_tyopl of SOME(c,tyop)
+             => TypeBasePure.put_boolify(c,boolify_eqs) info
+           | NONE => (HOL_MESG
+                      ("Can't find boolify constant for"^tyname);
+                      raise ERR "build_tyinfos" "")
+         end
+     in
+       ins_boolify tyinfo (TypeBasePure.ORIG def) ::
+       map (C ins_boolify (TypeBasePure.COPY (first_tyname,def))) rst
+     end
+     handle HOL_ERR _ => tyinfol);
+
+fun add_boolify tyinfol =
+  if List.exists (Option.isSome o TypeBasePure.boolify_of0) tyinfol then tyinfol
+  else
+    let
+      val db = TypeBase.theTypeBase ()
+      val recursion = TypeBasePure.axiom_of (hd tyinfol)
+    in
+      case define_boolify recursion db of SOME s
+        => insert_boolify s tyinfol
+      | NONE => (HOL_MESG "Couldn't define boolify function"; tyinfol)
+    end;
+
+val () = TypeBase.register_update_fn add_boolify;
+
+end
