src/Boolify/src/PreListBoolify.sig
@@ -1,0 +1,6 @@
+(* ========================================================================= *)
+(* FILLING IN "BOOLIFY" ENTRIES IN THE TYPEBASE FOR TYPES BUILT BEFORE LISTS *)
+(* Created by Joe Hurd and Konrad Slind, July 2002                           *)
+(* ========================================================================= *)
+
+signature PreListBoolify = sig end
