src/Boolify/test/datatypes.sml
@@ -1,0 +1,760 @@
+(* ========================================================================= *)
+(* Some (mutually, nested) recursive types from various sources, collected   *)
+(* by jrh.                                                                   *)
+(* Additions by Joe Hurd, June 2002.                                         *)
+(* ========================================================================= *)
+
+val () =
+  loadPath :=
+  ["../../../../ptr/hol/src/datatype/", "../../../../ptr/hol/src/list/src",
+   "../../../../ptr/hol/src/tfl/src", "../../../../ptr/hol/src/Boolify/src"] @
+  !loadPath;
+
+app load ["Datatype", "listTheory", "PreListBoolify"];
+
+fun first_token (QUOTE s :: _) = hd (String.tokens Char.isSpace s);
+val size_of = Lib.total TypeBase.size_of;
+val boolify_of = Lib.total TypeBase.boolify_of;
+
+val Hol_datatype =
+  fn q =>
+  let
+    val () = Lib.try (Count.apply Datatype.Hol_datatype) q
+    val tyname = first_token q
+  in
+    (tyname, size_of tyname, boolify_of tyname)
+  end;
+
+(* ------------------------------------------------------------------------- *)
+(* Very small examples to test basic functionality of datatype package.      *)
+(* ------------------------------------------------------------------------- *)
+
+Hol_datatype `NumBool = Num of num | Bool of bool`;
+
+Hol_datatype
+  `NumBoolNums = Num of num | Bool of bool | Nums of num list`;
+
+Hol_datatype `NTree = Tree of NTree list`;
+
+(* ------------------------------------------------------------------------- *)
+(* Miscellaneous examples.                                                   *)
+(* ------------------------------------------------------------------------- *)
+
+Hol_datatype
+         `Term = Var of 'A => 'B 
+               | App of bool => Termlist;
+      Termlist = Emp 
+               | Consp of Term => Termlist`;
+
+Hol_datatype
+      `List = Nil 
+            | Cons of 'A => List`;
+
+Hol_datatype
+    `Btree = Lf of 'A 
+           | Nd of 'B => Btree => Btree`;
+
+Hol_datatype
+    `Command = Assign of ind => Express
+             | If of Express => Command
+             | Ite of Express => Command => Command
+             | While of Express => Command
+             | Do of Command => Express;
+
+     Express = Constant of num
+             | Variable of ind
+             | Summ of Express => Express
+             | Product of Express => Express`;
+
+Hol_datatype
+    `testa = empty_testa 
+           | cons_testa of testa => testb;
+     testb = contentb of 'L => testc;
+     testc = connection of 'M => testa`;
+
+Hol_datatype
+    `atexp = Varb of ind 
+           | Let of dec => exp;
+
+       exp = Exp1 of atexp 
+           | Exp2 of exp => atexp 
+           | Exp3 of match;
+
+     match = Match1 of rule 
+           | Matches of rule => match;
+
+     rule  = Rule of pat => exp;
+       dec = Val of valbind 
+           | Local of dec => dec 
+           | Decs of dec => dec;
+
+   valbind = Single of pat => exp 
+           | Multi of pat => exp => valbind 
+           | Rec of valbind;
+
+       pat = Wild 
+           | Varpat of ind`;
+
+Hol_datatype
+     `tri = ONE | TWO | THREE`;
+
+(* ------------------------------------------------------------------------- *)
+(* A couple from Steve Brackin's work.                                       *)
+(* ------------------------------------------------------------------------- *)
+
+Hol_datatype
+      `Steve0 = X1  | X2  | X3  | X4  | X5  | X6  | X7  | X8  | X9  | X10 |
+                X11 | X12 | X13 | X14 | X15 | X16 | X17 | X18 | X19 | X20 |
+                X21 | X22 | X23 | X24 | X25 | X26 | X27 | X28 | X29 | X30 | 
+                X31 | X32 | X33 | X34`;
+
+Hol_datatype
+    `TY1 = NoF__ 
+         | Fk__ of 'A => TY2;
+
+     TY2 = Ta__   of bool 
+         | Td__   of bool 
+         | Tf__   of TY1 
+         | Tk__   of bool 
+         | Tp__   of bool
+         | App__  of 'A => TY1 => TY2 => TY3 
+         | Pair__ of TY2 => TY2;
+
+     TY3 = NoS__ 
+         | Fresh__        of TY2 
+         | Trustworthy__  of 'A
+         | PrivateKey__   of 'A => 'B => 'C 
+         | PublicKey__    of 'A => 'B => 'C
+         | Conveyed__     of 'A => TY2 
+         | Possesses__    of 'A => TY2 
+         | Received__     of 'A => TY2 
+         | Recognizes__   of 'A => TY2 
+         | Sends__        of 'A => TY2 => 'B 
+         | SharedSecret__ of 'A => TY2 => 'B
+         | Believes__     of 'A => TY3 
+         | And__          of TY3 => TY3
+         | NeverMalFromSelf__ of 'A => 'B => TY2`;
+
+(* ------------------------------------------------------------------------- *)
+(* Some with nesting of various kinds, plus required auxiliaries.            *)
+(* ------------------------------------------------------------------------- *)
+
+Hol_datatype `fot = aVar of 'a 
+                  | bApp of 'b => fot list`;
+
+Hol_datatype
+   `term = Vari of ind
+         | Fni of ind => term list`;
+
+Hol_datatype
+  `bintree = Leafb 
+           | Branchb of bintree # bintree`;
+
+Hol_datatype
+  `etree = Terminal 
+         | Nonterminal of num + etree`;
+
+Hol_datatype
+  `ptree = Only of ptree option`;
+
+Hol_datatype
+  `biterm = Variab of ind
+          | Fnapp of biterm list + biterm list`;
+
+Hol_datatype
+  `triterm = Var0 of ind
+           | Fun2 of triterm list + triterm list
+           | Fun1 of triterm list`;
+
+Hol_datatype
+    `xtree = Leafx of 'A
+           | Branchx of xtree list`;
+
+Hol_datatype
+  `array = Arry of num => 'A list`;
+
+Lib.try Hol_datatype 
+  `value = Integer of num
+         | Boolean of bool
+         | List of value list
+         | Tree of value xtree
+         | Array of value array`;
+
+Hol_datatype
+  `simper = Leaves of 'a => 'b
+          | Bough of simper xtree`;
+
+Lib.try Hol_datatype  (* used to fail *)
+  `simper = Leaves of 'A => 'B
+          | Bough of simper xtree`;
+
+Hol_datatype
+  `command 
+       = Assignment of num list # expression list
+       | Sequence   of command list
+   ;
+   expression 
+       = Numeral of num
+       | Plus    of expression # expression
+       | Valof   of command`;
+
+
+Hol_datatype
+  `mutual = Mutual of 'A => mutual => 'D => otherone 
+          | Friend of 'D => otherone;
+ otherone = Great of 'C 
+          | Expectations of mutual => otherone`;
+
+(* loops? *)
+Hol_datatype
+  `groof = Wu of bool
+         | Wibble of ('A,groof,'L)mutual
+         | Wobble of groof => groof`;
+
+(* loops? *)
+Hol_datatype
+  `zonk = Stonk of ((zonk,pink,'A)mutual)list # expression
+        | Tonk of zonk => pink list
+        | Honk of num;
+   pink = Floyd of zonk # pink
+        | Purple of num
+        | Rain of 'A # pink`;
+
+Hol_datatype `T1 = CONSTR1 of 'a`;
+
+Lib.try 
+Hol_datatype `T2 = CONSTR2 of T3 list => 'a T1
+                 ;
+              T3 = CONSTR31 of 'a T1
+                 | CONSTR32 of T2
+                 | CONSTR33 of 'b`;
+
+Hol_datatype `T4 = CONSTR4 of ('a,'b)T2 set`;
+
+Hol_datatype `ty1 = C1 of 'a 
+                  | C2 of ty2 option
+               ;
+              ty2 = C3 of 'b
+                  | C4 of ty1 list option`;
+
+delete_type "exp"; scrub();
+Hol_datatype
+        `exp = VAR of 'a
+             | IF  of bexp => exp => exp
+             | APP of 'b => exp list
+          ;
+        bexp = EQ  of exp => exp
+             | LEQ of exp => exp
+             | AND of bexp => bexp
+             | OR  of bexp => bexp
+             | NOT of bexp`;
+
+(*---------------------------------------------------------------------------
+   Example from Peter Homeier (tweaked)
+ ---------------------------------------------------------------------------*)
+
+
+Hol_datatype
+
+       (* obj ::= x | [li=mi] i in 1..n |  a.l | a.l:=m *)
+
+        `obj  = OVAR of 'a
+              | OBJ of (string # method) list
+              | INVOKE of obj => string
+              | UPDATE of obj => string => method ;
+
+        (* method ::= sigma x. o *)
+
+          method = SIGMA of 'a => obj` ;
+
+val REM_ALL_def = 
+ Define
+  `(REM_ALL x [] = []) /\
+   (REM_ALL x (h::t) = if x=h then REM_ALL x t else h::REM_ALL x t)`;
+
+val LDIFF_def = 
+ xDefine "LDIFF"
+  `(LDIFF L [] = L) /\
+   (LDIFF L (h::t) = LDIFF (REM_ALL h L) t)`;
+
+set_fixity "LDIFF" (Infixl 500);
+
+val FV_object = 
+ xDefine "FV_object"
+     `(FV_obj (OVAR x)        = [x])
+ /\   (FV_obj (OBJ d)         = FV_dict d)
+ /\   (FV_obj (INVOKE o1 l)   = FV_obj o1)
+ /\   (FV_obj (UPDATE o1 l m) = APPEND (FV_obj o1) (FV_method m))
+ /\   (FV_dict (e::es)        = APPEND (FV_entry e) (FV_dict es))
+ /\   (FV_dict  []            = [])
+ /\   (FV_entry (l, m)        = FV_method m)
+ /\   (FV_method (SIGMA x o1) = (FV_obj o1) LDIFF [x])`;
+
+
+(*---------------------------------------------------------------------------
+   Another example from Peter Homeier.
+ ---------------------------------------------------------------------------*)
+
+Hol_datatype
+        `(* vexp ::= n | x | SUC v | v+v | v-v | v*v | f (v1,...,vn)  *)
+
+          vexp = ANUM of num
+               | AVAR of string
+               | ASUC of vexp
+               | APLUS of vexp => vexp
+               | AMINUS of vexp => vexp
+               | AMULT of vexp => vexp
+               | ACONDV of aexp => vexp => vexp
+               | ACALL of string => vexp list ;
+
+       (* aexp ::= true | false | v=v | v<v | vs<<vs |
+                   a/\a | a\/a | ~a | a==>a | a=b |
+                   (a=>a|a) | !x.a | ?x.a                  *)
+
+          aexp = ATRUE
+               | AFALSE
+               | AEQ of vexp => vexp
+               | ALESS of vexp => vexp
+               | ALLESS of vexp list => vexp list
+               | AAND of aexp => aexp
+               | AOR of aexp => aexp
+               | ANOT of aexp
+               | AIMP of aexp => aexp
+               | AEQB of aexp => aexp
+               | ACOND of aexp => aexp => aexp
+               | AFORALL of string => aexp
+               | AEXISTS of string => aexp`;
+
+(* ------------------------------------------------------------------------- *)
+(* 68000 instruction set.                                                    *)
+(* ------------------------------------------------------------------------- *)
+
+Hol_datatype `Size = Byte | Word | Long`;
+
+Hol_datatype
+  `DataRegister 
+       = RegD0
+       | RegD1
+       | RegD2
+       | RegD3
+       | RegD4
+       | RegD5
+       | RegD6
+       | RegD7`;
+
+Hol_datatype
+  `AddressRegister 
+          = RegA0
+          | RegA1
+          | RegA2
+          | RegA3
+          | RegA4
+          | RegA5
+          | RegA6
+          | RegA7`;
+
+Hol_datatype
+ `DataOrAddressRegister
+               = data of DataRegister
+               | address of AddressRegister`;
+
+Hol_datatype
+    `Condition 
+         = Hi
+         | Ls
+         | Cc
+         | Cs
+         | Ne
+         | Eq
+         | Vc
+         | Vs
+         | Pl
+         | Mi
+         | Ge
+         | Lt
+         | Gt
+         | Le`;
+
+Hol_datatype
+ `AddressingMode 
+        = immediate of  num
+        | direct of DataOrAddressRegister
+        | indirect of AddressRegister
+        | postinc of AddressRegister
+        | predec of AddressRegister
+        | indirectdisp of num => AddressRegister
+        | indirectindex of num => AddressRegister => 
+                           DataOrAddressRegister => Size
+        | absolute of num
+        | pcdisp of num
+        | pcindex of num => DataOrAddressRegister => Size`;
+
+(* Elsa et al. package:
+    60 Meg.     runtime: 819.080s,    gctime: 101.500s,     systime: 0.780s.
+
+   JRH package: runtime: 3680.900s,    gctime: 1113.220s,     systime: 5.040s.
+*)
+Hol_datatype
+ `M68kInstruction
+    = ABCD of AddressingMode => AddressingMode
+    | ADD of Size => AddressingMode => AddressingMode
+    | ADDA of Size => AddressingMode => AddressRegister
+    | ADDI of Size => num => AddressingMode
+    | ADDQ of Size => num => AddressingMode
+    | ADDX of Size => AddressingMode => AddressingMode
+    | AND of Size => AddressingMode => AddressingMode
+    | ANDI of Size => num => AddressingMode
+    | ANDItoCCR of num
+    | ANDItoSR of num
+    | ASL of Size => AddressingMode => DataRegister
+    | ASLW of AddressingMode
+    | ASR of Size => AddressingMode => DataRegister
+    | ASRW of AddressingMode
+    | Bcc of Condition => Size => num
+    | BTST of Size => AddressingMode => AddressingMode
+    | BCHG of Size => AddressingMode => AddressingMode
+    | BCLR of Size => AddressingMode => AddressingMode
+    | BSET of Size => AddressingMode => AddressingMode
+    | BRA of Size => num
+    | BSR of Size => num
+    | CHK of AddressingMode => DataRegister
+    | CLR of Size => AddressingMode
+    | CMP of Size => AddressingMode => DataRegister
+    | CMPA of Size => AddressingMode => AddressRegister
+    | CMPI of Size => num => AddressingMode
+    | CMPM of Size => AddressRegister => AddressRegister
+    | DBT of DataRegister => num
+    | DBF of DataRegister => num
+    | DBcc of Condition => DataRegister => num
+    | DIVS of AddressingMode => DataRegister
+    | DIVU of AddressingMode => DataRegister
+    | EOR of Size => DataRegister => AddressingMode
+    | EORI of Size => num => AddressingMode
+    | EORItoCCR of num
+    | EORItoSR of num
+    | EXG of DataOrAddressRegister => DataOrAddressRegister
+    | EXT of Size => DataRegister
+    | ILLEGAL
+    | JMP of AddressingMode
+    | JSR of AddressingMode
+    | LEA of AddressingMode => AddressRegister
+    | LINK of AddressRegister => num
+    | LSL of Size => AddressingMode => DataRegister
+    | LSLW of AddressingMode
+    | LSR of Size => AddressingMode => DataRegister
+    | LSRW of AddressingMode
+    | MOVE of Size => AddressingMode => AddressingMode
+    | MOVEtoCCR of AddressingMode
+    | MOVEtoSR of AddressingMode
+    | MOVEfromSR of AddressingMode
+    | MOVEtoUSP of AddressingMode
+    | MOVEfromUSP of AddressingMode
+    | MOVEA of Size => AddressingMode => AddressRegister
+    | MOVEMto of Size => AddressingMode => DataOrAddressRegister list
+    | MOVEMfrom of Size => DataOrAddressRegister list => AddressingMode
+    | MOVEP of Size => AddressingMode => AddressingMode
+    | MOVEQ of num => DataRegister
+    | MULS of AddressingMode => DataRegister
+    | MULU of AddressingMode => DataRegister
+    | NBCD of AddressingMode
+    | NEG of Size => AddressingMode
+    | NEGX of Size => AddressingMode
+    | NOP
+    | NOT of Size => AddressingMode
+    | OR of Size => AddressingMode => AddressingMode
+    | ORI of Size => num => AddressingMode
+    | ORItoCCR of num
+    | ORItoSR of num
+    | PEA of AddressingMode
+    | RESET
+    | ROL of Size => AddressingMode => DataRegister
+    | ROLW of AddressingMode
+    | ROR of Size => AddressingMode => DataRegister
+    | RORW of AddressingMode
+    | ROXL of Size => AddressingMode => DataRegister
+    | ROXLW of AddressingMode
+    | ROXR of Size => AddressingMode => DataRegister
+    | ROXRW of AddressingMode
+    | RTE
+    | RTR
+    | RTS
+    | SBCD of AddressingMode => AddressingMode
+    | ST of AddressingMode
+    | SF of AddressingMode
+    | Scc of Condition => AddressingMode
+    | STOP of num
+    | SUB of Size => AddressingMode => AddressingMode
+    | SUBA of Size => AddressingMode => AddressingMode
+    | SUBI of Size => num => AddressingMode
+    | SUBQ of Size => num => AddressingMode
+    | SUBX of Size => AddressingMode => AddressingMode
+    | SWAP of DataRegister
+    | TAS of AddressingMode
+    | TRAP of num
+    | TRAPV
+    | TST of Size => AddressingMode
+    | UNLK of AddressRegister`;
+
+
+(* ------------------------------------------------------------------------- *)
+(* Example from Myra: part of the syntax of SML.                             *)
+(* ------------------------------------------------------------------------- *)
+
+Hol_datatype
+  `string = EMPTY_STRING 
+          | CONS_STRING of num => string`;
+
+Hol_datatype
+  `strid = STRID of string;
+   var = VAR of string;
+   con = CON of string;
+   scon = SCINT of num  (* was int *)
+        | SCSTR of string;
+   excon = EXCON of string;
+   label = LABEL of string`;
+
+Hol_datatype
+  `nonemptylist = Head_and_tail of 'A => 'A list`;
+
+Hol_datatype
+  `long = BASE of 'A | QUALIFIED of strid => long`;
+
+
+(* runtime on sole: 1251.940s,    gctime: 176.740s,     systime: 1.080s. *)
+
+Hol_datatype
+  `atpat_e = WILDCARDatpat_e
+           | SCONatpat_e   of scon
+           | VARatpat_e    of var
+           | CONatpat_e    of con long
+           | EXCONatpat_e  of excon long
+           | RECORDatpat_e of patrow_e option
+           | PARatpat_e    of pat_e;
+
+   patrow_e = DOTDOTDOT_e
+            | PATROW_e of label => pat_e => patrow_e option;
+
+   pat_e = ATPATpat_e   of atpat_e
+         | CONpat_e     of con long => atpat_e
+         | EXCONpat_e   of excon long => atpat_e
+         | LAYEREDpat_e of var => pat_e;
+
+   conbind_e = CONBIND_e of con => conbind_e option;
+
+   datbind_e = DATBIND_e of conbind_e => datbind_e option;
+
+   exbind_e = EXBIND1_e of excon => exbind_e option
+            | EXBIND2_e of excon => excon long => exbind_e option;
+
+   atexp_e = SCONatexp_e   of scon
+           | VARatexp_e    of var long
+           | CONatexp_e    of con long
+           | EXCONatexp_e  of excon long
+           | RECORDatexp_e of exprow_e option
+           | LETatexp_e    of dec_e => exp_e
+           | PARatexp_e    of exp_e;
+
+   exprow_e = EXPROW_e of label => exp_e => exprow_e option;
+
+   exp_e = ATEXPexp_e  of atexp_e
+         | APPexp_e    of exp_e => atexp_e
+         | HANDLEexp_e of exp_e => match_e
+         | RAISEexp_e  of exp_e
+         | FNexp_e     of match_e;
+
+   match_e = MATCH_e of mrule_e => match_e option;
+
+   mrule_e = MRULE_e of pat_e => exp_e;
+
+   dec_e = VALdec_e      of valbind_e
+         | DATATYPEdec_e of datbind_e
+         | ABSTYPEdec_e  of datbind_e => dec_e
+         | EXCEPTdec_e   of exbind_e
+         | LOCALdec_e    of dec_e => dec_e
+         | OPENdec_e     of (strid long) nonemptylist
+         | EMPTYdec_e
+         | SEQdec_e      of dec_e => dec_e;
+
+   valbind_e = PLAINvalbind_e of pat_e => exp_e => valbind_e option
+             | RECvalbind_e   of valbind_e`;
+
+(* ------------------------------------------------------------------------- *)
+(* Example from Daryl: a Verilog grammar.                                    *)
+(* ------------------------------------------------------------------------- *)
+
+Hol_datatype
+  `Source_text
+     = module of string => string list => Module_item list
+     | Source_textMeta of string;
+  Module_item
+     = declaration of Declaration
+     | initial of Statement
+     | always of Statement
+     | assign of Lvalue => Expression
+     | Module_itemMeta of string;
+  Declaration
+     = reg_declaration of Range option => string list
+     | net_declaration of Range option => string list
+     | input_declaration of Range option => string list
+     | output_declaration of Range option => string list
+     | DeclarationMeta of string;
+  Range = range of Expression => Expression 
+        | RangeMeta of string;
+  Statement
+     = clock_statement of Clock => Statement_or_null
+     | blocking_assignment of Lvalue => Expression
+     | non_blocking_assignment of Lvalue => Expression
+     | conditional_statement of Expression => Statement_or_null 
+                                => Statement_or_null option
+     | case_statement of Expression => Case_item list
+     | while_loop of Expression => Statement
+     | repeat_loop of Expression => Statement
+     | for_loop of Lvalue => Expression => Expression 
+                   => Lvalue => Expression => Statement
+     | forever_loop of Statement
+     | disable of string
+     | seq_block of string option => Statement list
+     | StatementMeta of string;
+  Statement_or_null = statement of Statement 
+                    | null_statement 
+                    | Statement_or_nullMeta of string;
+  Clock
+     = posedge of string
+     | negedge of string
+     | clock of string
+     | ClockMeta of string;
+  Case_item
+     = case_item of Expression list => Statement_or_null
+     | default_case_item of Statement_or_null
+     | Case_itemMeta of string;
+  Expression
+     = plus    of Expression => Expression
+     | minus   of Expression => Expression
+     | lshift  of Expression => Expression
+     | rshift  of Expression => Expression
+     | lt      of Expression => Expression
+     | leq     of Expression => Expression
+     | gt      of Expression => Expression
+     | geq     of Expression => Expression
+     | logeq   of Expression => Expression
+     | logneq  of Expression => Expression
+     | caseeq  of Expression => Expression
+     | caseneq of Expression => Expression
+     | bitand  of Expression => Expression
+     | bitxor  of Expression => Expression
+     | bitor   of Expression => Expression
+     | logand  of Expression => Expression
+     | logor   of Expression => Expression
+     | conditional of Expression => Expression => Expression
+     | positive  of Primary
+     | negative  of Primary
+     | lognot    of Primary
+     | bitnot    of Primary
+     | reducand  of Primary
+     | reducxor  of Primary
+     | reducor   of Primary
+     | reducnand of Primary
+     | reducxnor of Primary
+     | reducnor  of Primary
+     | primary   of Primary
+     | ExpressionMeta of string;
+  Primary
+     = primary_number of Number
+     | primary_IDENTIFIER of string
+     | primary_bit_select of string => Expression
+     | primary_part_select of string => Expression => Expression
+     | primary_gen_bit_select of Expression => Expression
+     | primary_gen_part_select of Expression => Expression => Expression
+     | primary_concatenation of Concatenation
+     | primary_multiple_concatenation of Multiple_concatenation
+     | brackets of Expression
+     | PrimaryMeta of string;
+  Lvalue
+     = lvalue of string
+     | lvalue_bit_select of string => Expression
+     | lvalue_part_select of string => Expression => Expression
+     | lvalue_concatenation of Concatenation
+     | LvalueMeta of string;
+  Number
+     = decimal of string
+     | based of string option => string
+     | NumberMeta of string;
+  Concatenation
+     = concatenation of Expression list
+     | ConcatenationMeta of string;
+  Multiple_concatenation
+     = multiple_concatenation of Expression => Expression list
+     | Multiple_concatenationMeta of string;
+  meta
+     = Meta_Source_text of Source_text
+     | Meta_Module_item of Module_item
+     | Meta_Declaration of Declaration
+     | Meta_Range of Range
+     | Meta_Statement of Statement
+     | Meta_Statement_or_null of Statement_or_null
+     | Meta_Clock of Clock
+     | Meta_Case_item of Case_item
+     | Meta_Expression of Expression
+     | Meta_Primary of Primary
+     | Meta_Lvalue of Lvalue
+     | Meta_Number of Number
+     | Meta_Concatenation of Concatenation
+     | Meta_Multiple_concatenation of Multiple_concatenation`;
+
+(* ------------------------------------------------------------------------- *)
+(* Various sizes of enumerated type.                                         *)
+(* ------------------------------------------------------------------------- *)
+
+Hol_datatype `Enum1 = one`;
+
+Hol_datatype `Enum2 = one | two`;
+
+Hol_datatype `Enum3 = one | two | three`;
+
+Hol_datatype `Enum4 = one | two | three | four`;
+
+Hol_datatype `Enum5 = one | two | three | four | five`;
+
+Hol_datatype `Enum6 = one | two | three | four | five | six`;
+
+Hol_datatype `Enum7 = one | two | three | four | five | six | seven`;
+
+Hol_datatype
+`Enum30 =
+  one | two | three | four | five | six | seven | eight | nine | ten
+| eleven | twelve | thirteen | fourteen | fifteen | sixteen | seventeen
+| eighteen | nineteen | twenty | twentyone | twentytwo | twentythree
+| twentyfour | twentyfive | twentysix | twentyseven | twentyeight
+| twentynine | thirty`;
+
+Hol_datatype
+`Enum31 =
+  one | two | three | four | five | six | seven | eight | nine | ten
+| eleven | twelve | thirteen | fourteen | fifteen | sixteen | seventeen
+| eighteen | nineteen | twenty | twentyone | twentytwo | twentythree
+| twentyfour | twentyfive | twentysix | twentyseven | twentyeight
+| twentynine | thirty | thirtyone`;
+
+Hol_datatype
+`Enum32 =
+  one | two | three | four | five | six | seven | eight | nine | ten
+| eleven | twelve | thirteen | fourteen | fifteen | sixteen | seventeen
+| eighteen | nineteen | twenty | twentyone | twentytwo | twentythree
+| twentyfour | twentyfive | twentysix | twentyseven | twentyeight
+| twentynine | thirty | thirtyone | thirtytwo`;
+
+Hol_datatype
+`Enum33 =
+  one | two | three | four | five | six | seven | eight | nine | ten
+| eleven | twelve | thirteen | fourteen | fifteen | sixteen | seventeen
+| eighteen | nineteen | twenty | twentyone | twentytwo | twentythree
+| twentyfour | twentyfive | twentysix | twentyseven | twentyeight
+| twentynine | thirty | thirtyone | thirtytwo | thirtythree`;
+
+Hol_datatype
+`Enum34 =
+  one | two | three | four | five | six | seven | eight | nine | ten
+| eleven | twelve | thirteen | fourteen | fifteen | sixteen | seventeen
+| eighteen | nineteen | twenty | twentyone | twentytwo | twentythree
+| twentyfour | twentyfive | twentysix | twentyseven | twentyeight
+| twentynine | thirty | thirtyone | thirtytwo | thirtythree | thirtyfour`;
