src/Boolify/test/test.sml
@@ -1,0 +1,87 @@
+(* ========================================================================= *)
+(* TEST SUITE FOR HOL BOOLIFICATION.                                         *)
+(* Created by Joe Hurd, July 2002                                            *)
+(* ========================================================================= *)
+
+val () =
+  loadPath :=
+  ["../../datatype/", "../../list/src", "../../tfl/src", "../src"] @
+  !loadPath;
+
+app load
+["sumTheory", "Datatype", "listTheory", "Boolify", "bossLib"];
+
+(* ------------------------------------------------------------------------- *)
+(* Helper functions.                                                         *)
+(* ------------------------------------------------------------------------- *)
+
+fun first_token (QUOTE s :: _) = hd (String.tokens Char.isSpace s)
+  | first_token _ = "if_you_can_read_this_then_first_token_probably_failed";
+val size_of = Lib.total TypeBase.size_of;
+val boolify_of = Lib.total TypeBase.boolify_of;
+
+val Hol_datatype =
+  fn q =>
+  let
+    val () = Lib.try (Count.apply Datatype.Hol_datatype) q
+    val tyname = first_token q
+  in
+    (tyname, size_of tyname, boolify_of tyname)
+  end;
+
+fun boolify tm = 
+  let
+    val db = TypeBase.theTypeBase()
+    val f = TypeBasePure.type_boolify db (type_of tm)
+  in
+    (*CONV_RULE (REDEPTH_CONV pairLib.PAIRED_BETA_CONV)*)
+    (bossLib.EVAL (mk_comb (f, tm)))
+  end;
+
+(* ------------------------------------------------------------------------- *)
+(* Example datatypes to test boolification.                                  *)
+(* ------------------------------------------------------------------------- *)
+
+try Hol_datatype `NumBool0 = Num0 of num | Bool0 of bool`;
+
+try Hol_datatype `NumBoolNums = Num of num | Bool of bool | Nums of num list`;
+
+try Hol_datatype `NTree = Tree of NTree list`;
+
+try Hol_datatype `List = Nil | Cons of 'A => List`;
+
+try Hol_datatype `tri = ONE | TWO | THREE`;
+
+try Hol_datatype
+  `command 
+       = Assignment of num list # expression list
+       | Sequence   of command list
+   ;
+   expression 
+       = Numeral of num
+       | Plus    of expression # expression
+       | Valof   of command`;
+
+try Hol_datatype
+        `exp = VAR of 'a
+             | IF  of bexp => exp => exp
+             | APP of 'b => exp list
+          ;
+        bexp = EQ  of exp => exp
+             | LEQ of exp => exp
+             | AND of bexp => bexp
+             | OR  of bexp => bexp
+             | NOT of bexp`;
+
+(* ------------------------------------------------------------------------- *)
+(* Boolification of terms.                                                   *)
+(* ------------------------------------------------------------------------- *)
+
+try boolify (Term `[(1,2,3,4) ; (5,6,7,8)]`);
+try boolify (Term `(SOME F, 123, [F;T])`);
+try boolify (Term `[]:num list`);
+try boolify (Term `[1; 2; 3]`);
+try boolify (Term `(Num 1, Nums [2; 3])`);
+try boolify (Term `Tree [Tree []; Tree [Tree []; Tree []]; Tree []]`);
+try boolify (Term `[INL TWO; INR (Bool0 T)]`);
+try boolify (Term `Assignment ([1; 2], [Numeral 1])`);
