src/datatype/Datatype.sml
@@ -99,30 +99,6 @@ fun tysize_env db =
      Option.map fst o 
      Option.composePartial (TypeBasePure.size_of, TypeBasePure.get db)
 
-local open Portable
-      fun num_variant vlist v =
-        let val counter = ref 0
-            val names = map (fst o dest_var) vlist
-            val (Name,Ty) = dest_var v
-            fun pass str =
-               if mem str names
-               then (inc counter; pass (Name^Lib.int_to_string(!counter)))
-               else str
-        in mk_var(pass Name,  Ty)
-        end
-in
-fun mk_tyvar_boolify vty (V,away) =
-  let val fty = vty --> mk_type ("list", [bool])
-      val v = num_variant away (mk_var("f", fty))
-  in (v::V, v::away)
-  end
-end;
-
-fun tyboolify_env db = 
-     Option.map fst o 
-     Option.composePartial (TypeBasePure.boolify_of, TypeBasePure.get db)
-
-
 (*---------------------------------------------------------------------------*
  * Term size, as a function of types. The function gamma maps type           *
  * operator "ty" to term "ty_size". Types not registered in gamma are        *
@@ -267,188 +243,6 @@ fun define_size ax db =
  handle HOL_ERR _ => NONE
 end;
 
-(*---------------------------------------------------------------------------*
-  Term boolification, another type-based translation.
- *---------------------------------------------------------------------------*)
-
-fun bool_list () = mk_type ("list", [bool]);
-  
-fun bool_nil () = mk_thy_const {Thy = "list", Name = "NIL", Ty = bool_list ()};
-  
-fun bool_cons () =
-  mk_thy_const
-  {Thy = "list", Name = "CONS", Ty = bool --> bool_list () --> bool_list ()};
-fun mk_bool_cons (x, y) = list_mk_comb (bool_cons (), [x, y]);
-  
-fun bool_append () =
-  mk_thy_const
-  {Thy = "list", Name = "APPEND",
-   Ty = bool_list () --> bool_list () --> bool_list ()};
-fun mk_bool_append (x, y) = list_mk_comb (bool_append (), [x, y]);
-
-local
-  fun booll _ _ Nil 0 = [Nil]
-    | booll ConsT ConsF Nil n =
-    let val l = booll ConsT ConsF Nil (n div 2)
-    in map ConsT l @ map ConsF l
-    end;
-in
-  fun bool_lists n =
-    List.take
-    (booll (curry mk_bool_cons T) (curry mk_bool_cons F) (bool_nil ()) (n - 1),
-     n);
-end;
-
-local fun drop [] ty = fst(dom_rng ty)
-        | drop (_::t) ty = drop t (snd(dom_rng ty));
-      fun Kzero ty = mk_abs(mk_var("v",ty), bool_nil ())
-      fun OK f ty M =
-         let val (Rator,Rand) = dest_comb M
-         in (Rator=f) andalso is_var Rand andalso (type_of Rand = ty)
-         end
-in
-fun tyboolify (theta,omega,gamma) clause ty =
- case theta ty
-  of SOME fvar => fvar
-   | NONE =>
-      case omega ty
-       of SOME (_,[]) => raise ERR "tyboolify" "bug: no assoc for nested"
-        | SOME (_,[(f,szfn)]) => szfn
-        | SOME (_,alist) => snd
-             (first (fn (f,sz) => Lib.can (find_term(OK f ty)) (rhs clause))
-                  alist)
-        | NONE =>
-           let val (Tyop,Args) = dest_type ty
-           in case gamma Tyop
-               of SOME f =>
-                   let val vty = drop Args (type_of f)
-                       val sigma = Type.match_type vty ty
-                    in list_mk_comb(inst sigma f,
-                                map (tyboolify (theta,omega,gamma) clause) Args)
-                    end
-                | NONE => Kzero ty
-             end
-
-fun type_boolify db ty =
-  let fun theta ty = if is_vartype ty then SOME (Kzero ty) else NONE
-      fun omega ty = NONE
-  in
-    tyboolify (theta,omega,tyboolify_env db) ty
-  end
-end;
-
-fun dupls [] (C,D) = (rev C, rev D)
-  | dupls (h::t) (C,D) = dupls t (if mem h t then (C,h::D) else (h::C,D));
-
-fun crunch [] = []
-  | crunch ((x,y)::t) =
-    let val key = #1(dom_rng(type_of x))
-        val (yes,no) = partition (fn(x,_) => (#1(dom_rng(type_of x))=key)) t
-    in (key, (x,y)::yes)::crunch no
-    end;
-
-fun unflatten f =
-  let
-    fun h (x, s) =
-      let
-        val k = f x
-      in
-        case List.partition (equal k o fst) s of ([(_, l)], r)
-          => (k, x :: l) :: r
-        | _ => (k, [x]) :: s
-      end
-  in
-    rev o map (rev o snd) o foldl h []
-  end;
-
-fun define_boolify ax db =
- let val dtys = Prim_rec.doms_of_tyaxiom ax  (* primary types in axiom *)
-     val tyvars = Lib.U (map (snd o dest_type) dtys)
-     val (_, abody) = strip_forall(concl ax)
-     val (exvs, ebody) = strip_exists abody
-     (* list of all constructors with arguments *)
-     val conjl = strip_conj ebody
-     val bare_conjl = map (snd o strip_forall) conjl
-     val capplist = map (rand o lhs) bare_conjl
-     val def_name = fst(dest_type(type_of(hd capplist)))
-     (* 'a -> bool list variables : boolify functions for type variables *)
-     val fparams = rev(fst(rev_itlist mk_tyvar_boolify tyvars
-                             ([],free_varsl capplist)))
-     val fparams_tyl = map type_of fparams
-     fun proto_const n ty =
-         mk_var(n, itlist (curry op-->) fparams_tyl (ty --> bool_list ()))
-     fun tyop_binding ty =
-       let val root_tyop = fst(dest_type ty)
-       in (root_tyop, (ty, proto_const(root_tyop^"_to_bool") ty))
-       end
-     val tyvar_map = zip tyvars fparams
-     val tyop_map = map tyop_binding dtys
-     fun theta tyv =
-          case assoc1 tyv tyvar_map
-           of SOME(_,f) => SOME f
-            | NONE => NONE
-     val type_boolify_env = tyboolify_env db
-     fun gamma str =
-          case assoc1 str tyop_map
-           of NONE  => type_boolify_env str
-            | SOME(_,(_, v)) => SOME v
-     (* now the ugly nested map *)
-     val head_of_clause = head o lhs o snd o strip_forall
-     fun is_dty M = mem(#1(dom_rng(type_of(head_of_clause M)))) dtys
-     val (dty_clauses,non_dty_clauses) = partition is_dty bare_conjl
-     val dty_fns = fst(dupls (map head_of_clause dty_clauses) ([],[]))
-     fun dty_boolify ty =
-        let val (d,r) = dom_rng ty
-        in list_mk_comb(proto_const(fst(dest_type d)^"_to_bool") d,fparams)
-        end
-     val dty_map = zip dty_fns (map (dty_boolify o type_of) dty_fns)
-     val non_dty_fns = fst(dupls (map head_of_clause non_dty_clauses) ([],[]))
-     fun nested_binding (n,f) =
-        let val name = String.concat[def_name,Lib.int_to_string n,"_to_bool"]
-            val (d,r) = dom_rng (type_of f)
-            val proto_const = proto_const name d
-        in (f, list_mk_comb (proto_const,fparams))
-       end
-     val nested_map0 = map nested_binding (enumerate 1 non_dty_fns)
-     val nested_map1 = crunch nested_map0
-     fun omega ty = assoc1 ty nested_map1
-     val boolifyr = tyboolify(theta,omega,gamma)
-     fun mk_app cl v = mk_comb(boolifyr cl (type_of v), v)
-     val fn_i_map = dty_map @ nested_map0
-     fun clause (bl, cl) =
-         let val (fn_i, capp) = dest_comb (lhs cl)
-         in
-         mk_eq(mk_comb(assoc fn_i fn_i_map, capp),
-               end_itlist (curry mk_bool_append)
-               (bl :: map (mk_app cl) (snd(strip_comb capp))))
-(*
-               case snd(strip_comb capp)
-                of [] => bool_nil ()
-                 | L  => end_itlist (curry mk_bool_append)
-                         (mk_bool_cons (T, bool_nil ())::map (mk_app cl) L))
-*)
-         end
-     val bare_conjls = unflatten (rator o lhs) bare_conjl
-     val annot_conjs =
-       flatten (map (fn l => zip (bool_lists (length l)) l) bare_conjls)
-     val pre_defn0 = list_mk_conj (map clause annot_conjs)
-     val nil_rws =
-       [CONJUNCT1 (DB.fetch "list" "APPEND"), DB.fetch "list" "APPEND_NIL"]
-     val pre_defn1 = rhs(concl   (* remove zero additions *)
-                      ((DEPTH_CONV BETA_CONV THENC
-                        Rewrite.PURE_REWRITE_CONV nil_rws) pre_defn0))
-     val defn = new_recursive_definition
-                 {name=def_name^"_to_bool_def",
-                  rec_axiom=ax, def=pre_defn1}
-     val cty = (I##(type_of o last)) o strip_comb o lhs o snd o strip_forall
-     val ctyl = Lib.mk_set (map cty (strip_conj (concl defn)))
-     val const_tyl = gather (fn (c,ty) => mem ty dtys) ctyl
-     val const_tyopl = map (fn (c,ty) => (c,fst(dest_type ty))) const_tyl
- in
-    SOME {def=defn,const_tyopl=const_tyopl}
- end
- handle HOL_ERR _ => NONE;
-
 (*---------------------------------------------------------------------------
            Basic datatype definition support
  ---------------------------------------------------------------------------*)
@@ -550,7 +344,6 @@ fun build_enum_tyinfo (tyname, ast) =
 fun build_enum_tyinfos astl = map build_enum_tyinfo astl
 
 
-
 (*---------------------------------------------------------------------------
     Returns a list of tyinfo thingies
  ---------------------------------------------------------------------------*)
@@ -576,27 +369,6 @@ local
          map (C insert_size (TypeBasePure.COPY (first_tyname,def))) rst
        end
        handle HOL_ERR _ => tyinfol);
-
-  fun insert_boolify {def, const_tyopl} tyinfol =
-    (case tyinfol of [] => raise ERR "build_tyinfos" "empty tyinfo list"
-     | tyinfo::rst =>
-       let
-         val first_tyname = TypeBasePure.ty_name_of tyinfo
-         fun insert_boolify info boolify_eqs =
-           let
-             val tyname = TypeBasePure.ty_name_of info
-           in
-             case assoc2 tyname const_tyopl of SOME(c,tyop)
-               => TypeBasePure.put_boolify(c,boolify_eqs) info
-             | NONE => (HOL_MESG
-                        ("Can't find boolify constant for"^tyname);
-                        raise ERR "build_tyinfos" "")
-           end
-       in
-         insert_boolify tyinfo (TypeBasePure.ORIG def) ::
-         map (C insert_boolify (TypeBasePure.COPY (first_tyname,def))) rst
-       end
-       handle HOL_ERR _ => tyinfol);
 in
   fun build_tyinfos db {induction,recursion} =
     let
@@ -606,14 +378,7 @@ in
     in
       case define_size recursion db
         of NONE => (HOL_MESG "Couldn't define size function"; tyinfol)
-      | SOME s =>
-          let
-            val tyinfol = insert_size s tyinfol
-          in
-            case define_boolify recursion db of SOME s
-              => insert_boolify s tyinfol
-            | NONE => (HOL_MESG "Couldn't define boolify function"; tyinfol)
-          end
+      | SOME s => insert_size s tyinfol
     end;
 end;
 
@@ -659,9 +424,8 @@ end (* local *)
 
  ---------------------------------------------------------------------------*)
 
-fun adjoin {ax,case_def,case_cong,induction,nchotomy,
-            one_one,distinct,boolify,size} record_rw_names 
-  =
+fun adjoin [] = raise ERR "Hol_datatype" "no tyinfos"
+  | adjoin (string_etc0 :: strings_etc) =
  adjoin_to_theory
    {sig_ps = NONE,
     struct_ps = SOME
@@ -676,7 +440,7 @@ fun adjoin {ax,case_def,case_cong,induction,nchotomy,
                in S ("         size="^line); NL();
                   S ("                   "^s^"),")
                end
-          fun do_boolify NONE = (S "         boolify = NONE,"; NL())
+          fun do_boolify NONE = S "         boolify = NONE,"
             | do_boolify (SOME (c,s)) =
                let val strc = String.concat
                      ["(", term_to_string c, ") ",type_to_string (type_of c)]
@@ -684,31 +448,41 @@ fun adjoin {ax,case_def,case_cong,induction,nchotomy,
                in S ("         boolify="^line); NL();
                   S ("                   "^s^"),")
                end
-          fun do_simpls() = (S "["; app S (Lib.commafy record_rw_names); S "]")
-          fun do_field_rws() =
-            if null record_rw_names then (S " tyinfo0;")
-            else (NL();S "       (TypeBasePure.put_simpls ("; do_simpls();
-                  S " @ TypeBasePure.simpls_of tyinfo0) tyinfo0);")
+          fun do_simpls record_rw_names =
+            (S "["; app S (Lib.commafy record_rw_names); S "]")
+          fun do_field_rws record_rw_names =
+            if null record_rw_names then ()
+            else (S "      val tyinfo0 = put_simpls (";
+                  do_simpls record_rw_names;
+                  S " @ simpls_of tyinfo0) tyinfo0"; NL())
+          fun do_string_etc ({ax,case_def,case_cong,induction,nchotomy,
+            one_one,distinct,boolify,size}, record_rw_names) =
+            (S "    let";                                               NL();
+             S "      open TypeBasePure";                               NL();
+             S "      val tyinfo0 = mk_tyinfo";                         NL();
+             S("        {ax="^ax^",");                                  NL();
+             S("         case_def="^case_def^",");                      NL();
+             S("         case_cong="^case_cong^",");                    NL();
+             S("         induction="^induction^",");                    NL();
+             S("         nchotomy="^nchotomy^",");                      NL();
+             do_size size;                                              NL();
+             do_boolify boolify;                                        NL();
+             S("         one_one="^one_one^",");                        NL();
+             S("         distinct="^distinct^"}");                      NL();
+             do_field_rws record_rw_names;
+             S "      val () = computeLib.write_datatype_info tyinfo0"; NL();
+             S "    in";                                                NL();
+             S "      tyinfo0";                                         NL();
+             S "    end")
       in
-        S "val _ =";                                      NL();
-        S "   let open TypeBasePure ";                    NL();
-        S "       val tyinfo0 = mk_tyinfo";               NL();
-        S ("        {ax="^ax^",");                        NL();
-        S ("         case_def="^case_def^",");            NL();
-        S ("         case_cong="^case_cong^",");          NL();
-        S ("         induction="^induction^",");          NL();
-        S ("         nchotomy="^nchotomy^",");            NL();
-        do_size size;                                     NL();
-        do_boolify boolify;                               NL();
-        S ("         one_one="^one_one^",");              NL();
-        S ("         distinct="^distinct^"}");            NL();
-        S "   in";                                        NL();
-        S "    TypeBase.write "; do_field_rws();          NL();
-        S "    computeLib.write_datatype_info tyinfo0";   NL();
-        S "   end;";                                      NL()
+        S "val _ =";                                                    NL();
+        S "  TypeBase.write [";                                         NL();
+        do_string_etc string_etc0;
+        app (fn se => (S ","; NL(); do_string_etc se)) strings_etc;     NL();
+        S "  ];";                                                       NL()
       end)};
 
-fun write_tyinfo (tyinfo, record_rw_names) =
+fun write_tyinfo tyinfo =
  let open TypeBasePure
      fun name s = ty_name_of tyinfo ^ s
      val one_one_name =
@@ -764,24 +538,27 @@ fun write_tyinfo (tyinfo, record_rw_names) =
             => SOME (tm, "COPY ("^Lib.quote s^","^s^"_to_bool_def)")
        end
  in
-  adjoin{ax        = axiom_name,
-         induction = induction_name,
-         case_def  = name"_case_def",
-         case_cong = case_cong_name,
-         nchotomy  = nchotomy_name,
-         size      = size_info,
-         boolify   = boolify_info,
-         one_one   = one_one_name,
-         distinct  = distinct_name}
-     record_rw_names
+   {ax        = axiom_name,
+    induction = induction_name,
+    case_def  = name"_case_def",
+    case_cong = case_cong_name,
+    nchotomy  = nchotomy_name,
+    size      = size_info,
+    boolify   = boolify_info,
+    one_one   = one_one_name,
+    distinct  = distinct_name}
  end;
 
+val write_tyinfos = adjoin o map (write_tyinfo ## I);
 
-
-fun persistent_tyinfo (x as (tyinfo,_)) =
-   (TypeBase.write tyinfo;
-    computeLib.write_datatype_info tyinfo;
-    write_tyinfo x)
+fun persistent_tyinfo tyinfos_etc =
+  let
+    val (tyinfos, etc) = unzip tyinfos_etc
+    val tyinfos = TypeBase.write tyinfos
+    val () = app computeLib.write_datatype_info tyinfos
+  in
+    write_tyinfos (zip tyinfos etc)
+  end;
 
 fun Hol_datatype q = let
   val tyinfos_etc = primHol_datatype (TypeBase.theTypeBase()) q
@@ -789,9 +566,9 @@ fun Hol_datatype q = let
   val message = "Defined "^(if length tynames > 1 then "types" else "type")^
                 ": "^String.concat (Lib.commafy tynames)
 in
-  List.app persistent_tyinfo tyinfos_etc;
+  persistent_tyinfo tyinfos_etc;
   HOL_MESG message
-end handle ? => Raise (wrap_exn "Datatype" "Hol_datatype" ?);
+end handle ? as HOL_ERR _ => Raise (wrap_exn "Datatype" "Hol_datatype" ?);
 
 
 
